ABCVoting/Impossibilities/Peters/BaseCase.lean
@@ -58,8 +58,8 @@ lemma W_P₁_eq_W_P₁' (f : ABCRule V C k) (hres : f.IsResolute) :
   simpa [W] using this
 
 theorem base_case_impossible
-    (f : ABCRule V C k) (hwf : f.IsWellFormed) (hres : f.IsResolute)
-    (hprop : f.SatisfiesProportionality) (hsp : f.SatisfiesResoluteStrategyproofness) :
+    (f : ABCRule V C k) (hwf : f.IsWellFormedOnPlentiful) (hres : f.IsResolute)
+    (hprop : f.SatisfiesProportionality) (hsp : Peters.SatisfiesResoluteStrategyproofnessOnPlentiful f) :
     False := by
   have hc : (2 : C) ∈ W f hres P₁ P₁_proper := c_in_W_P₁ f hres hprop
   have hd : (3 : C) ∈ W f hres P₁ P₁_proper := d_in_W_P₁ f hres hprop
